theories/ftlr/Restrict.v
@@ -5,6 +5,7 @@ From stdpp Require Import base.
 From cap_machine.ftlr Require Import ftlr_base interp_weakening.
 From cap_machine.rules Require Import rules_base rules_Restrict.
 From cap_machine Require Export logrel register_tactics.
+From cap_machine Require Export stdpp_extra.
 
 Section fundamental.
   Context {Σ:gFunctors} {memg:memG Σ} {regg:regG Σ} {sealsg: sealStoreG Σ}
@@ -19,31 +20,22 @@ Section fundamental.
   Lemma PermPairFlows_interp_preserved p p' b e a widc :
     p <> E ->
     p <> IE ->
+    p' <> IE ->
     PermFlowsTo p' p = true →
-    (□ ▷ (∀ a0 a1 a2 a3 a4 w',
-             full_map a0
-          -∗ (∀ (r1 : RegName) v, ⌜r1 ≠ PC⌝ → ⌜r1 ≠ idc⌝ → ⌜a0 !! r1 = Some v⌝ → (fixpoint interp1) v)
-          -∗ registers_mapsto (<[idc:=w']> (<[PC:=WCap a1 a2 a3 a4]> a0))
+    (□ ▷ (∀ regs' p' b' e' a' widc',
+             full_map regs'
+          -∗ (∀ (r : RegName) v, ⌜r ≠ PC⌝ → ⌜r ≠ idc⌝ → ⌜regs' !! r = Some v⌝ → (fixpoint interp1) v)
+          -∗ registers_mapsto (<[idc:=widc']> (<[PC:=WCap p' b' e' a']> regs'))
           -∗ na_own logrel_nais ⊤
-          -∗ □ (fixpoint interp1) (WCap a1 a2 a3 a4)
-          -∗ □ (fixpoint interp1) w'
+          -∗ □ (fixpoint interp1) (WCap p' b' e' a')
+          -∗ □ (fixpoint interp1) widc'
           -∗ interp_conf)) -∗
     (fixpoint interp1) widc -∗
     (fixpoint interp1) (WCap p b e a) -∗
     (fixpoint interp1) (WCap p' b e a).
   Proof.
-    intros HpnotE HpnotIE Hp. iIntros "#IH HIDC HA".
-    iApply (interp_weakening with "[IH]") ; eauto ; try solve_addr.
-  Qed.
-
-  Lemma match_perm_with_E_rewrite:
-    forall (A: Type) p (a1 a2: A),
-      match p with
-      | E => a1
-      | _ => a2
-      end = if (perm_eq_dec p E) then a1 else a2.
-  Proof.
-    intros. destruct (perm_eq_dec p E); destruct p; auto; congruence.
+    intros HpnotE HpnotIE Hp'notIE Hp. iIntros "#IH HIDC HA".
+    iApply (interp_weakening with "IH HIDC") ; eauto ; try solve_addr.
   Qed.
 
   Lemma restrict_case (r : leibnizO Reg) (p : Perm)
@@ -54,6 +46,9 @@ Section fundamental.
     iIntros "#IH #Hinv_pc #Hinv_idc #Hinva #Hreg #[Hread Hwrite] Hown Ha HP Hcls HPC HIDC Hmap".
     iInsertList "Hmap" [idc;PC].
 
+
+    (* TODO we need to do some manipulation in the resources here *)
+
     iApply (wp_Restrict with "[$Ha $Hmap]"); eauto.
     { simplify_map_eq; auto. }
     { rewrite /subseteq /map_subseteq /set_subseteq_instance. intros rr _.
@@ -62,18 +57,16 @@ Section fundamental.
     }
 
     iIntros "!>" (regs' retv). iDestruct 1 as (HSpec) "[Ha Hmap]".
-    destruct HSpec as [ * Hdst ? Hz Hfl HincrPC | * Hdst Hz Hfl HincrPC | ].
+    destruct HSpec as [ * Hdst HnE HnIE Hz Hfl HincrPC | * Hdst Hz Hfl HincrPC | ].
     { apply incrementPC_Some_inv in HincrPC as (p''&b''&e''&a''& ? & HPC & Z & Hregs') .
 
       assert (a'' = a ∧ b'' = b ∧ e'' = e) as (-> & -> & ->).
-      { destruct (decide (PC = dst)) ; simplify_map_eq; auto;
-        [ rewrite lookup_insert in Hdst; rewrite lookup_insert in HPC |
-        (rewrite lookup_insert_ne in HPC ; [rewrite lookup_insert in HPC|auto])] ; by simplify_eq.
-      }
+      { destruct (decide (PC = dst)) ; simplify_map_eq; auto. }
 
       iApply wp_pure_step_later; auto.
       iMod ("Hcls" with "[HP Ha]");[iExists w;iFrame|iModIntro].
       iNext; iIntros "_".
+
       (* TODO rewrite regs' to match with the induction hypothesis *)
       iApply ("IH" $! regs' with "[%] [] [Hmap] [$Hown]").
       { cbn. intros. subst regs'. by repeat (apply lookup_insert_is_Some'; right). }
@@ -81,12 +74,14 @@ Section fundamental.
         subst regs'.
         rewrite lookup_insert_ne in Hvs; auto.
         destruct (decide (ri = dst)).
-        { subst ri.
-          rewrite lookup_insert_ne in Hdst; auto.
-          rewrite lookup_insert_ne in Hdst; auto.
-          rewrite lookup_insert in Hvs; inversion Hvs. simplify_eq.
+        { simplify_map_eq.
           unshelve iSpecialize ("Hreg" $! dst _ _ _ Hdst); eauto.
-          iApply (interp_weakening with "IH Hreg"); auto; solve_addr. }
+          destruct (decide ((decodePerm n) = IE)) as [ Heq | Hneq]; simplify_eq ; cycle 1.
+           { iApply (interp_weakening with "IH Hreg") ; auto; solve_addr. }
+           rewrite Heq; rewrite Heq in Hfl; clear Heq.
+           admit. (* TODO lemma in case of IE *)
+
+        }
         { repeat (rewrite lookup_insert_ne in Hvs); auto.
           iApply "Hreg"; auto. } }
         { subst regs'. rewrite insert_insert. iApply "Hmap". }
